\documentclass{article}
\usepackage[pdftex]{graphicx}
\begin{document}

Setting, $y=4x^2+5x$ we get,
\[
8x^2+10x+3=\frac{1}{4x^2+7x+3}
\Leftrightarrow 2y+3=\frac{1}{y+2x+3}
\Leftrightarrow 2y^2+(4x+9)y+(6x+8)=0
\]
Using qudratic formula for, $y$ we get,
$y=\frac{-(4x+9) \pm \sqrt{(4x+9)^2-8(6x+8)}}{4}$

Putting the value of $y$ and after some calculation we get,
$\Leftrightarrow 16x^2+24x+9=\pm \sqrt{16x^2+24x+17}$
Here, $16x^2+24x+9=(4x+3)^2>0$ 
So,$\begin{equation}16x^2+24x+9=\sqrt{16x^2+24x+17}\end{equation}$
(Here is assume that we want the solution for $x \in \mathbb{R}$, if it is not the case we can do in the same way)
Setting $(4x+3)^2=z$ in $(1)$we get,
$z=\sqrt{z+8}$
Solving this we get,
$z=\frac{1+\sqrt{33}}{2}$
And putting the value of, $z$ we get,
$x=\frac{-3 \pm \sqrt{\frac{1+\sqrt{33}}{2}}}{4}$
\end{document}